Change some definitions for [Label]

src/SemDet.v
@@ -3,7 +3,7 @@ Require Import Permutation.
 Require Import Common FMap Syntax Semantics.
 
 Inductive step_det (sys: System) : State Msg -> Label -> State Msg -> Prop :=
-| SdSlt: forall s, step_det sys s emptyLabel s
+| SdSlt: forall s, step_det sys s LblEmpty s
 | SdInt: forall oss oims obj idx mf os pos fmsg fpmsg fidx fchn outs,
     In obj (sys_objs sys) ->
     idx = obj_idx obj ->
@@ -19,7 +19,7 @@ Inductive step_det (sys: System) : State Msg -> Label -> State Msg -> Prop :=
     outs = pmsg_outs fpmsg os (msg_value fmsg) ->
 
     step_det sys {| st_oss := oss; st_msgs := oims |}
-             (buildLabel nil (Some fmsg) (extOuts sys outs))
+             (LblHdl fmsg (extOuts sys outs))
              {| st_oss := oss +[ idx <- pos ];
                 st_msgs := distributeMsgs (intOuts sys outs) oims |}
 | SdExt: forall from emsgs oss oims,
@@ -27,7 +27,7 @@ Inductive step_det (sys: System) : State Msg -> Label -> State Msg -> Prop :=
     emsgs <> nil ->
     SubList (map (fun m => mid_to (msg_id m)) emsgs) (indicesOf sys) ->
     step_det sys {| st_oss := oss; st_msgs := oims |}
-             (buildLabel emsgs None nil)
+             (LblIns emsgs)
              {| st_oss := oss; st_msgs := distributeMsgs emsgs oims |}.
 
 Definition steps_det := steps step_det.
